examples/ghc/theories/CoreInduct.v
@@ -15,9 +15,9 @@ Require Import Proofs.Core.
 Set Bullet Behavior "Strict Subproofs".
 
 
-Lemma core_induct :
-  forall (e : CoreExpr)
-  (P : CoreExpr -> Prop)
+Lemma core_induct' {b} :
+  forall (e : Expr b)
+  (P : Expr b -> Prop)
   (HVar  : forall v, P (Mk_Var v))
   (HLit  : forall l, P (Lit l))
   (HApp  : forall e1 e2, P e1 -> P e2 -> P (App e1 e2))
@@ -46,7 +46,7 @@ Proof.
   * apply HApp; apply IH.
   * apply HLam; apply IH.
   * apply HLet.
-    - destruct b as [v rhs|pairs]; simpl.
+    - destruct b0 as [v rhs|pairs]; simpl.
       + simpl.
         apply IH.
       + induction pairs as [|[v rhs] pairs']; simpl.
@@ -71,6 +71,28 @@ Proof.
   * apply HType.
   * apply HCoercion.
 Qed.
+
+Lemma core_induct :
+  forall (e : CoreExpr)
+  (P : CoreExpr -> Prop)
+  (HVar  : forall v, P (Mk_Var v))
+  (HLit  : forall l, P (Lit l))
+  (HApp  : forall e1 e2, P e1 -> P e2 -> P (App e1 e2))
+  (HLam  : forall v e, P e -> P (Lam v e))
+  (HLet  : forall binds body,
+      (match binds with
+       | NonRec v rhs => P rhs
+       | Rec pairs    => (forall v rhs, In (v, rhs) pairs -> P rhs)
+       end) ->
+      P body ->
+      P (Let binds body))
+  (HCase : forall scrut bndr ty alts, P scrut -> (forall dc pats rhs, In (dc, pats ,rhs) alts -> P rhs) -> P (Case scrut bndr ty alts))
+  (HCast : forall e co, P e -> P (Cast e co))
+  (HTick : forall tickish e, P e -> P (Tick tickish e))
+  (HType : forall ty, P (Type_ ty))
+  (HCoercion : forall co, P (Coercion co)),
+  P e.
+Proof. exact core_induct'. Qed.
 
 Section CoreLT.
   Context {v : Type}.
